First changes to GenericTyping for locally irr types.

theories/BasicAst.v
@@ -1,8 +1,0 @@
-(** * LogRel.BasicAst: definitions preceding those of the AST of terms: sorts, binder annotations… *)
-From Coq Require Import String Bool.
-From LogRel.AutoSubst Require Import core unscoped.
-
-Inductive sort :=
-  | set : sort.
-
-Definition sort_of_product (s s' : sort) := set.
